Moved the type msg of messages from UCBasicTypes.ec to UCCore.ec, in preparation for the UC DSL debugger, in which port will be concrete, but messages will be symbolic.

common/UCBasicTypes.ec
@@ -2,7 +2,7 @@
 
 (* Exports standard theories, encoding and partial decoding pairs
    (EPDPs), the type univ plus a number of EPDPs with target univ;
-   defines addresses, ports and messages *)
+   defines addresses and ports *)
 
 (* standard theories *)
 
@@ -49,17 +49,28 @@ hint rewrite epdp : valid_epdp_addr_univ.
 
 (* ports - pairs of functionality addresses and port indices
 
-   a functionality's ports are divided between its different parties
+   port indices are used to implement naming schemes for messages
+   (see UCCore.ec) with identical destination addresses
 
-   adversaries can handle multiple port indices, and each simulator
-   has a single, distinct port index
+   when a direct message comes to a real functionality, the message's
+   destination port index is used to determine which party it should
+   be sent to
 
-   ([], 0) is the root port of the environment *)
+   when an adversarial message comes to a real functionality, the
+   message's destination port index is used to determine which party
+   it should be sent to (the same port may correspond to different
+   parties in direct and adversarial messages)
+
+   adversaries can handle multiple port indices, corresponding to
+   different ideal functionalities or real functionality parties
+
+   each simulator handles a single port index, distinct from those
+   of all other simulators *)
 
 type port = addr * int.
 
 op epdp_port_univ : (port, univ) epdp =
-  epdp_pair_univ epdp_addr_univ epdp_int_univ.
+  epdp_pair_univ (epdp_list_univ epdp_int_univ) epdp_int_univ.
 
 lemma valid_epdp_port_univ : valid_epdp epdp_port_univ.
 proof.
@@ -71,38 +82,9 @@ hint rewrite epdp : valid_epdp_port_univ.
 
 (* in UC DSL, envport is a keyword, and so cannot be used as an
    ordinary identifier. in DSL specs, it has type port -> bool, but in
-   the generated EasyCrypt code it has type _addr -> addr -> bool, and
+   the generated EasyCrypt code it has type addr -> addr -> bool, and
    is applied to the address of the functionality and adversary - in
    addition to the port expression *)
 
 op envport (self adv : addr, pt : port) : bool =
   ! self <= pt.`1 /\ ! adv <= pt.`1  /\ pt <> ([], 0).
-
-(* messages have modes:
-
-     * direct - supplying functionality inputs, consuming their
-         outputs
-
-     * adversarial - communication between functionalties and
-         adversaries/simulators, communication between different
-         adversaries/simulators, and communication between
-         environments and adversaries/simulators *)
-
-type mode = [
-  | Dir  (* direct *)
-  | Adv  (* adversarial *)
-].
-
-lemma not_dir (mod : mode) :
-  mod <> Dir <=> mod = Adv.
-proof. by case mod. qed.
-
-lemma not_adv (mod : mode) :
-  mod <> Adv <=> mod = Dir.
-proof. by case mod. qed.
-
-(* a message has the form (mod, pt1, pt2, tag, u), for a mode mod, a
-   destination port pt1, a source port pt2, an integer tag (used to
-   ensure certain messages are distinct), and a universe value u *)
-
-type msg = mode * port * port * int * univ.
